StandardLibrary/test/VarEncode32.dfy
@@ -32,10 +32,10 @@ module {:options "-functionSyntax:4"} VarEncode32Test {
         var val := currPo2 + i;
         if (val < UINT32_LIMIT) {
           CheckValue(val as uint32);
-          currPo2 := currPo2 * 2;
           assert currPo2 >= 1024;
         }
       }
+      currPo2 := currPo2 * 2;
     }
   }
 }
